% --------------------------------------------------------------------
\begin{tactic}[apply (p : proof-term)]{apply}
  \begin{tsyntax}[empty]{apply (p : proof-term)}
   If \tct{p} is a proof-term for the pattern (formula)
  \begin{center}
    \tct{forall (x1 : t1) ... (xn : tn), A1 -> ... -> An -> B}
  \end{center}
  \noindent then \tct{apply} tries to match B with the current G. If the
  match succeeds and leads to the full instantiation of the pattern,
  then the goal is replaced, after instantiation, with the $n$ subgoals
  \tct{A1, ..., An}.
  \end{tsyntax}
\end{tactic}
